    ## region upper concepts
## order ALPHA
@prefix dct:            <http://purl.org/dc/terms/> .
@prefix fno:            <https://w3id.org/function/ontology#> .
@prefix foaf:           <http://xmlns.com/foaf/0.1/> .
@prefix odrl:           <http://www.w3.org/ns/odrl/2/> .
@prefix org:            <http://www.w3.org/ns/org#> .
@prefix owl:            <http://www.w3.org/2002/07/owl#> .
@prefix prof:           <http://www.w3.org/ns/dx/prof/> .
@prefix role:           <http://www.w3.org/ns/dx/prof/role/> .
@prefix qudt:           <http://qudt.org/schema/qudt/> .
@prefix rdf:            <http://www.w3.org/1999/02/22-rdf-syntax-ns#> .
@prefix rdfs:           <http://www.w3.org/2000/01/rdf-schema#> .
@prefix sh:             <http://www.w3.org/ns/shacl#> .
@prefix skos:           <http://www.w3.org/2004/02/skos/core#> .
@prefix time:           <http://www.w3.org/2006/time#>.
@prefix unit:           <http://qudt.org/vocab/unit/> .
@prefix vann:           <http://purl.org/vocab/vann/> .
@prefix voaf:           <http://purl.org/vocommons/voaf#> .
@prefix void:           <http://rdfs.org/ns/void#> .
@prefix xsd:            <http://www.w3.org/2001/XMLSchema#> .
## endregion upper concepts

@prefix lds:            <https://github.com/nicosResearchAndDevelopment/LDS/> .

lds:ServiceInstance                         ## REM: abstract
    a                owl:Class ;
    rdfs:label       "Service Instance"@en ;
    rdfs:label       "Service Instanz"@de ;
    ## region skos
    a                skos:Concept ;
    skos:notation    "ServiceInstance"^^xsd:string ;
    skos:prefLabel   "Service Instance"^^xsd:string ;
    skos:inScheme    lds:Service ;
    skos:related     lds:ServiceConfiguration ;
    ## endregion skos
    rdfs:isDefinedBy lds: .

lds:serviceInstance
    a                owl:ObjectProperty ;
    rdfs:label       "Service Instanz"@en ;
    dct:description  """Property to bind a given Service Instance, 'lds:ServiceInstance'."""@en ;
    skos:notation    "serviceInstance"^^xsd:string ;
    skos:prefLabel   "Service Instance"^^xsd:string ;
    rdfs:range       lds:ServiceInstance ;
    rdfs:isDefinedBy lds: .

lds:ServiceConfiguration                    ## REM: abstract
    a                owl:Class ;
    rdfs:label       "Service Configuration"@en ;
    rdfs:label       "Service Konfiguration"@de ;
    ## region skos
    a                skos:Concept ;
    skos:notation    "ServiceConfiguration"^^xsd:string ;
    skos:prefLabel   "Service Configuration"^^xsd:string ;
    skos:related     lds:ServiceInstance ;
    ## endregion skos
    rdfs:isDefinedBy lds: .

lds:serviceConfiguration
    a                owl:ObjectProperty ;
    rdfs:label       "Service Konfiguration"@en ;
    dct:description  """Property to bind a given Service Configuration , 'lds:ServiceConfiguration' to a given Service Instance 'lds:ServiceInstance'."""@en ;
    skos:notation    "serviceConfiguration"^^xsd:string ;
    skos:prefLabel   "Service Configuration"^^xsd:string ;
    rdfs:range       lds:ServiceInstance ;
    rdfs:isDefinedBy lds: .

lds:agreementPolicy
    a                owl:ObjectProperty ;
    rdfs:label       "Agreement"@en ;
    ## region skos
    dct:description  """Property to bind a given Agreement , 'odrl:Agreement' to a given Service Configuration 'lds:ServiceConfiguration'."""@en ;
    skos:notation    "agreementPolicy"^^xsd:string ;
    skos:prefLabel   "Policy of Agreement"^^xsd:string ;
    ## endregion skos
    rdfs:domain      lds:ServiceConfiguration ;
    rdfs:range       odrl:Agreement ;
    rdfs:isDefinedBy lds: .

## EOF lds.service.instance.ttl
